fairness/locales_helpers.v
@@ -42,10 +42,12 @@ Section XX.
   Qed.
 
   Lemma locales_of_cfg_Some τ tp σ:
-    τ ∈ locales_of_cfg (tp, σ) -> is_Some (from_locale tp τ).
+    τ ∈ locales_of_cfg (tp, σ) <-> is_Some (from_locale tp τ).
   Proof.
     rewrite /locales_of_cfg. simpl. rewrite elem_of_list_to_set.
-    apply locales_of_list_from_locale_from'.
+    split. 
+    - apply locales_of_list_from_locale_from'.
+    - apply locales_of_list_from_locale_from. 
   Qed.
 
   Definition step_fork (c1 c2: cfg Λ): option (locale Λ) :=
